proof/correctness/Termination.ec
@@ -5,87 +5,40 @@ require import XMSS_IMPL XMSS_IMPL_PP Generic.
 
 from Jasmin require import JModel.
 
-(* Auxiliary Lemmas *)
-(* NOTE: Lemmas with admit are annotated with nosmt *)
+lemma to_of_int (i : int) : 0 <= i < W64.max_uint => to_uint ((of_int i))%W64 = i by move => ? ; smt(@W64).
 
-lemma lemma_1 (a b : int) :
-    a - b <= 0 => ! (b < a) by smt().
-
-lemma lemma_2 (a : int) (b : W64.t) :
-    0 <= a < W64.max_uint => 
-    a - to_uint b <= 0 => ! (b \ult W64.of_int a) by smt(@W64). 
-
-lemma lemma_3 (a : W64.t) (b : int) :
-    0 <= b < W64.max_uint => 
-    b - to_uint a <= 0 => ! (a \ult W64.of_int b) by smt(@W64).
-
-lemma nosmt lemma_4 (a b : W64.t) :
-    a - b \ule W64.zero => ! (b \ult a).
+lemma memcpy_ll : phoare [Memcpy._x_memcpy_u8u8 : 0 <= inlen < W64.max_uint ==> true] = 1%r.
 proof.
-admit. (* smt(@W64). fails *)
+proc.
+while (#pre /\ 0 <= to_uint i <= inlen) (inlen - to_uint i) ; auto => />.
+  - move => &hr. rewrite ultE of_uintK //= => *. rewrite to_uintD_small => /#.
+  - move => &hr ?????. rewrite ultE //= => *. rewrite to_of_int => /#. 
 qed.
 
-lemma nosmt lemma_5 (a b : W64.t) : 
-    to_uint (a - (b + W64.one)) < to_uint (a - b).
-proof.    
-admit.
+lemma ull_to_bytes_2_ll  : islossless Mp(Syscall).__ull_to_bytes_2 by proc ; while (true) (i - aux) ; by auto => /> /#.
+lemma ull_to_bytes_32_ll : islossless Mp(Syscall).__ull_to_bytes_32 by proc ; while (true) (i - aux) ; by auto => /> /#.
+
+lemma addr_to_bytes_ll : islossless Mp(Syscall).__addr_to_bytes.
+proc.
+while (true) (8 - i); last by auto => /> /#.
+auto => />.
+inline; by auto => /> /#.
 qed.
 
-lemma lemma_5_int (a b : int) : a - (b + 1) < (a - b) by smt().
-lemma lemma_6_int (a b : int) : a - (b + 1) < a - b by smt().
-
-lemma nosmt lemma_6_W32 (a b : W32.t) :
-    to_uint a - to_uint (b + W32.one) < to_uint a - to_uint b.
+lemma thash_f_ll : islossless Mp(Syscall)._thash_f.
 proof.
-admit. (* smt(@W32 lemma_6_int). *)
+proc.
+inline Mp(Syscall).__thash_f => //=.
+auto => />.
+while (0 <= to_uint i <= 32) (32 - to_uint i) ; auto => />.
+  - auto => /> &hr *. do split ; 1,2: by smt(@W64). rewrite to_uintD_small => /#.
+  - auto => /> *. split ; [ progress ; rewrite ultE => /# | auto ].
+  - call (addr_to_bytes_ll). inline Mp(Syscall).__set_key_and_mask ; auto => />. 
+    call (addr_to_bytes_ll) ; auto => />. 
+    call (ull_to_bytes_32_ll). auto => /> i. rewrite ultE /= => * /#.
 qed.
-
-lemma nosmt lemma_6_W64 (a b : W64.t) :
-    to_uint a - to_uint (b + W64.one) < to_uint a - to_uint b.
-proof.
-admit. (* smt(@W32 lemma_6_int). *)
-qed.
-
-lemma nosmt lemma_7 (a : int) (b : W64.t) : a - to_uint (b + W64.one) < a - to_uint b.
-proof.
-do rewrite /to_uint => //=.
-admit.
-qed.
-
-lemma lemma_8 (b : W64.t) : 32 - to_uint b <= 0 => ! (b \ult (of_int 32)%W64) by smt(@W64).
-lemma lemma_9 (a : W64.t) : 64 - to_uint a <= 0 => ! (a \ult (of_int 64)%W64) by smt(@W64).
-
-lemma nosmt lemma_10 (a : int) (b : W64.t) :
-    a - to_uint (b + W64.one) < a - to_uint b.
-proof.
-admit. (* smt(@W64). *)
-qed.
-
-lemma lemma_11 (a b : W64.t) : to_uint a - to_uint b <= 0 => ! (b \ult a) by smt(@W64).
-lemma nosmt lemma_12 (a : W64.t) : 64 - to_uint (a + W64.one) < 64 - to_uint a.
-proof.
-rewrite /to_uint /W64.one.
-simplify.
-admit.
-qed.
-
-lemma nosmt lemma_13 (a : int) (b : W64.t) : 
-    0 < a < W64.max_uint =>
-    a - to_uint (b + W64.one) < a - to_uint b. 
-proof.
-admit. (*  smt(@W64) fails *)
-qed.
-
-lemma nosmt lemma_14 (a : int) (b : W64.t) : a - to_uint b <= 0 => ! (b \ult (of_int a)%W64).
-proof.
-admit. (* smt(@W64). *)
-qed.
-
-lemma lemma_15 (a : W64.t) : 
-    a \ult (of_int 32)%W64 => 32 - to_uint (a + W64.one) < 32 - to_uint a by smt.
 
 (* Base w *)
-
 lemma base_w_ll : islossless BaseWGeneric.__base_w.
 proof.
 proc.
@@ -93,50 +46,6 @@ islossless.
 while (true) ((to_uint outlen) - (to_uint consumed)) ; [auto => /> *; smt(@W64) | skip => /> /#].
 qed.
 
-(*
-lemma base_w_ll (output : W32.t list, outlen : W64.t, input : W8.t list): 
-    W64.zero \ule outlen =>
-    phoare [BaseWGeneric.__base_w : arg=(output, outlen, input) ==> true] = 1%r.
-proof.
-move => outlen_ge0.
-proc.
-while (W64.zero \ule consumed{hr} /\ W64.zero \ule outlen{hr}) (to_uint (outlen - consumed)).
-auto => /> *. 
-do split ; [ smt(@W64) | smt(lemma_5) ]. (* lemma_5 is not proved *)
-(* Second subgoal *)
-auto => /> * ; smt(@W64).
-qed.
-*)
-
-(* Gen Chain *)
-lemma gen_chain_ll : islossless Mp(Syscall).__gen_chain.
-proof.
-proc ; inline*.
-islossless.
-  - while (true) ((to_uint t) - (to_uint i)) ; last by skip => /> * ; smt(@W64).
-    auto => />. islossless ; first by auto => /> ; smt(lemma_6_W32).
-      - while (true) (32 - to_uint i1) ; [auto => /> * ; smt(lemma_10) | skip => /> * ; smt(lemma_8)].
-      - while (true) (8 - i4) ; [auto => /# | skip => /> /#].
-      - while (true) (8 - i3) ; [auto => /# | skip => /> /#].
-      - while (true) (i2 - aux0) ; [auto => /> /# | skip => /> /#].
-  - while (true) ((to_uint inlen) - (to_uint i0)) ; [auto => /> * ; smt(lemma_6_W64) | skip => /> * ; smt(lemma_11)].
-qed.
-
-lemma gen_chain_inplace_ll : islossless Mp(Syscall).__gen_chain_inplace.
-proof.
-proc ; inline*.
-islossless.
-while (true) ((to_uint t) - (to_uint i)) ; last by skip => /> /#.
-auto => /> *. 
-islossless.
-  - auto => /> ; smt(lemma_6_W32).
-  - while (true) (32 - to_uint i0) ; [auto => /> * ; smt(lemma_7) | skip => /> * ; smt(@W64)].
-  - while (true) (8 - i3) ; [auto => /> * ; smt(@W64) | skip => /> /#].
-  - while (true) (8 - i2) ; [auto => /> /# | skip => /> /#].
-  - while (true) (i1 - aux0) ; [auto => /# | skip => /> /#].
-qed.
-
-(* Checksum *)
 lemma csum_ll : islossless Mp(Syscall).__csum.
 proof.
 proc.
@@ -148,72 +57,80 @@ qed.
 lemma checksum_ll : islossless Mp(Syscall).__wots_checksum.
 proof.
 proc.
-islossless.
-  - while (true) ((to_uint outlen) - (to_uint consumed)) ; [auto => /> * ; smt(lemma_6_W64) | skip => /> * ; smt(lemma_11)].
-  - while (true) (i - aux) ;  [auto => /> /# | skip => /#].
-  - while (true) (64 - to_uint i) ; [auto => /> * ; smt(lemma_12) | skip => /> ; smt(@W64)].
+auto => />.
+call (base_w_ll).
+call (ull_to_bytes_2_ll).
+auto => />.
+call (csum_ll).
+auto => /> .
+qed.
+
+(* Gen Chain *)
+lemma gen_chain_inplace_ll : islossless Mp(Syscall).__gen_chain_inplace.
+proof.
+proc.
+auto => />.
+(*
+while (0 <= to_uint i <= to_uint t) ((to_uint t) - (to_uint i)).
+  - auto => />. inline Mp(Syscall).__thash_f_ ;  auto => /> ; call(thash_f_ll).
+    inline. auto => /> &hr. rewrite ultE. rewrite to_uintD_small => //=. admit. progress. smt(). admit. idtac => //= /#.
+  - auto => /> &hr i. rewrite ultE -lezNgt => /#.
+*)
+admit.
+qed.
+
+lemma gen_chain_ll : islossless Mp(Syscall).__gen_chain by admit.
+
+(* Chain Lengths *)
+lemma chain_lengths_ll : islossless Mp(Syscall).__chain_lengths.
+proof.
+proc.
+auto => /> ; call (checksum_ll).
+auto => /> ; call (base_w_ll).
+auto => />.
 qed.
 
 (* Expand Seed *)
-lemma expand_seed_ll : islossless Mp(Syscall).__expand_seed_.
+lemma expand_seed_ll : islossless Mp(Syscall).__expand_seed.
 proof.
-proc ; inline*.
-islossless.  
-  - while (true) (67 - i); last by skip => /> /#. auto => /> *. while (true) (8 - i1) ; by auto => /> /#.
-  - while (true) (inlen - to_uint i0) ; [auto => /> * ; apply lemma_10 | skip => /> * ; smt(lemma_14)].
+proc.
+while (true) (67 - i) ; auto => />.
+  - call (addr_to_bytes_ll). inline. auto => /> /#.
+  - call (memcpy_ll). auto => />. inline ; auto => /> /#.
 qed.
 
 (* Pk Gen *)
 lemma pkgen_ll : islossless Mp(Syscall).__wots_pkgen.
 proof.
-proc ; inline*.
-islossless.
-(* 1 *)
-  - while (true) (67 - i) ; last by skip => /> /#. auto => /> *. islossless ; first by auto => /#.
-    - while (true) ((to_uint t) - (to_uint i1)) ; last by skip => /> * ; smt(lemma_11). auto => /> *. islossless.
-        - auto => /> * ; smt(lemma_6_W32).
-        - while (true) (32 - to_uint i4) ; [auto => /> * ; smt(lemma_15) | skip => /> * ; smt(lemma_8)].
-        - while (true) (8 - i7) ; [auto => /> /# | skip => /> /#].
-        - while (true) (8 - i6) ; [auto => /> /# | skip => /> /#].
-        - while (true) (i5 - aux3) ; [auto => /> /# | skip => /> /#].
-(* 2 *) 
-  - while (true) (67 - i0) ; last by skip => /> /#. auto =>  /> *. islossless ; first by smt().
-    while (true) (8 - i3) ; [auto => /> /# | skip => /> /#].
-(* 3 *)
-  - while (true) (inlen - to_uint i2); [auto => /> * ; smt(lemma_6_W64) | skip => /> * ; smt(lemma_14)].
+proc.
+while (true) (67 - i).
+  - auto => />. inline Mp(Syscall).__gen_chain_inplace_ ; inline Mp(Syscall)._gen_chain_inplace ; auto => />.
+    call (gen_chain_inplace_ll). inline. auto => /> /#.
+  - inline Mp(Syscall).__expand_seed_.
+    inline Mp(Syscall)._expand_seed ; auto => />.
+    call(expand_seed_ll) ; by auto => /> /#.
 qed.
 
 (* Sign *)
 lemma wots_sign_ll : islossless Mp(Syscall).__wots_sign.
 proof.
-proc ; inline*.
-islossless.
-(* 1 *)
-- while (true) (67 - i); last by skip => /> /#. auto => /> *. islossless; first by auto => /> /#.
-  while (true) ((to_uint t) - (to_uint i0)) ; last by skip => /> /#. auto => /> *. islossless.
-  - auto => /> * ; smt(lemma_6_W32).
-  - while (true) (32 - to_uint i4) ; [auto => /> * ; smt(lemma_7) | skip => /> * ; smt(lemma_8)].
-  - while (true) (i9 - 8); by admit.
-  - idtac. (* FIX HERE *)
-  - while (true) (i7 - aux4) ; by auto => /> /#.
-(* 2 *)
-- while (true) (67 - i1); last by skip => /#. auto => /> *. islossless; first by auto => /> /#.
-  while (true) (8 - i3) ; [auto => /> /# | skip => /> /#].
-(* 3 *)
-- while (true) (inlen - to_uint i2) ; [auto => /> * ; smt(lemma_10) | skip => /> * ; smt(lemma_14)].
-(* 4 *)
-- while (true) ((to_uint outlen1) - (to_uint consumed0)) ;  [auto => /> * ; smt(lemma_6_W64) | skip => /> * ; smt(lemma_11)].
-(* 5 *)
--  while (true) (i6 - aux3) ; [auto => /> /# | skip => /#].
-(* 6 *)
-- while (true) (64 - to_uint i5) ; [auto => /> * ; smt(lemma_12) | skip => /> * ; smt(lemma_9)].
-(* 7 *)
-- while (true) ((to_uint outlen) - (to_uint consumed)) ; [auto => /> * ; smt (lemma_6_W64) | skip => /> * ; smt(lemma_11)].
+proc.
+while (true) (67 - i).
+  - auto => />. inline Mp(Syscall).__gen_chain_inplace_ ; inline Mp(Syscall)._gen_chain_inplace ; auto => />.
+    call (gen_chain_inplace_ll). inline* ; auto => /> /#.
+  - inline Mp(Syscall).__expand_seed_ ; inline Mp(Syscall)._expand_seed ; auto => /> ; call(expand_seed_ll).
+    inline Mp(Syscall).__chain_lengths_ ; inline Mp(Syscall)._chain_lengths ; auto => />.
+    call(chain_lengths_ll) ; by auto => /> /#.
 qed.
 
 (* Pk from Sig *)
 lemma wots_pk_from_sig_ll : islossless Mp(Syscall).__wots_pk_from_sig.
 proof.
-proc ; inline*.
-admit.
+proc => //=.
+while (true) (67 - i).
+  - auto => />. inline Mp(Syscall).__gen_chain_ ; inline Mp(Syscall)._gen_chain ; auto => />.
+    call(gen_chain_ll); by inline ; auto => /> /#.
+  - inline Mp(Syscall).__chain_lengths_ ; inline Mp(Syscall)._chain_lengths ; auto => />.
+    call (chain_lengths_ll) ; by auto => /> /#.
 qed.
+
