scripts/run-all-tests.sh
@@ -1,0 +1,12 @@
+#!/bin/bash
+
+test_dirs=(
+    "wots"
+    "xmss"
+)
+
+for dir in ${test_dirs[@]}; do
+    make -C ../test/$dir clean
+    make -C ../test/$dir
+    make -C ../test/$dir run
+done
